coq-osiris/theories/lang/syntax.v
@@ -285,6 +285,8 @@ Inductive expr :=
 
   (* Creating a thread: [Thread.create f arg]. *)
   | EFork (e1 e2 : expr)
+  (* Waiting for another thread to terminate: [Thread.join th]. *)
+  | EJoin (e : expr)
 
 (* Field-expression pairs. *)
 
